arrived at point where need to change substitution

dev/lf/dot_top_bot.v
@@ -228,7 +228,7 @@ Inductive ty_trm : tymode -> submode -> ctx -> trm -> typ -> Prop :=
     ty_trm ty_general m2 G (trm_app (avar_f x) (avar_f z)) (open_typ z T)
 | ty_new_intro : forall L m1 m2 G T ds,
     (forall x, x \notin L ->
-      ty_defs (G & (x ~ open_typ x T)) (open_defs x ds) (open_typ x T)) ->
+      ty_defs (G & (x ~ open_typ x (typ_bnd T))) (open_defs x ds) (open_typ x T)) ->
     ty_trm m1 m2 G (trm_val (val_new T ds)) (typ_bnd T)
 | ty_new_elim : forall m2 G x m T,
     ty_trm ty_general m2 G (trm_var (avar_f x)) (typ_rcd (dec_trm m T)) ->
@@ -441,7 +441,7 @@ Proof.
     apply* H.
   + intros. subst.
     apply_fresh ty_new_intro as z; assert (zL: z \notin L) by auto.
-    - specialize (H z zL G1 G2 (G3 & z ~ open_typ z T)).
+    - specialize (H z zL G1 G2 (G3 & z ~ open_typ z (typ_bnd T))).
       repeat rewrite concat_assoc in H.
       apply* H.
   + intros. subst.
@@ -633,7 +633,7 @@ Proof.
     apply_fresh ty_new_intro as y; eauto;
     assert (y \notin L) as FrL by eauto.
     specialize (H y FrL).
-    specialize (H G1 (G2 & y ~ open_typ y T) x S).
+    specialize (H G1 (G2 & y ~ open_typ y (typ_bnd T)) x S).
     eapply H; eauto.
     rewrite concat_assoc. reflexivity.
     rewrite concat_assoc. reflexivity.
@@ -1062,9 +1062,12 @@ Proof.
     }
     rewrite <- A at 2. rewrite <- A at 3. rewrite <- A at 4.
     rewrite <- subst_open_commute_typ. rewrite <- subst_open_commute_defs.
-    assert (subst_ctx x y G2 & z ~ subst_typ x y (open_typ z T) = subst_ctx x y (G2 & z ~ open_typ z T)) as B. {
-      unfold subst_ctx. rewrite map_concat. rewrite map_single. reflexivity.
-    }
+    assert (z \notin L) by admit.
+    specialize (H z H0 G1 (G2 & z ~ open_typ z (typ_bnd T)) x). 
+    assert (subst_ctx x y G2 & z ~ open_typ (subst_fvar x y z) (typ_bnd (subst_typ x y T)) =
+            subst_ctx x y (G2 & z ~ open_typ z (typ_bnd T))) as B. {
+            unfold subst_ctx. rewrite map_concat. rewrite map_single. 
+            admit. }
     rewrite <- concat_assoc. rewrite B.
     apply H; eauto.
     rewrite concat_assoc. reflexivity.
@@ -1874,7 +1877,7 @@ Qed.
 (* ###################################################################### *)
 (** ** Narrowing *)
 
-
+(*
 Lemma narrowing: 
   (forall m1 m2 G' t S,
     ty_trm m1 m2 G' t S ->
@@ -1914,9 +1917,12 @@ Proof.
       auto. eapply weaken_subtyp. assumption. assumption.
     * apply binds_push_neq_inv in b. eapply weaken_ty_trm.
       constructor. assumption. assumption. assumption.
-  - 
+  - apply_fresh ty_all_intro as y.
+    assert (y \notin L) as Hy by auto.
+    specialize (t0 y Hy).
+    specialize (H y Hy).
 Admitted.
-
+*)
 
 Definition subenv(G1 G2: ctx) :=
   forall x T2, binds x T2 G2 ->
@@ -2017,7 +2023,7 @@ Lemma narrow_subtyping: forall G G' S U,
 Proof.
   intros. apply* narrow_rules.
 Qed.
-*)
+
 (* ###################################################################### *)
 (** * Has member *)
 
